Curify.lean
@@ -1,4 +1,4 @@
 import Curify.Basic
 import Curify.Core
-import Curify.Expr
 import Curify.Store
+import Curify.Expr
